translations/translation_utils.v
@@ -1,4 +1,4 @@
-Require Import Template.All.
+From Template Require Import All.
 Require Import List.
 Import ListNotations MonadNotation String.
 Open Scope string_scope.
@@ -53,14 +53,23 @@ Instance monad_exc : MonadExc tsl_error tsl_result :=
       end
   }.
 
+Definition lookup_tsl_table' E gr :=
+  match lookup_tsl_table E gr with
+  | Some t => ret t
+  | None => raise (TranslationNotFound (string_of_gref gr))
+  end.
 
 
-Class Translation := { tsl_id : ident -> ident ;
-                       tsl_tm : tsl_context -> term -> tsl_result term ;
-                       tsl_ty : tsl_context -> term -> tsl_result term ;
-                       tsl_ind : tsl_context -> kername -> kername -> mutual_inductive_body
-                            -> tsl_result (tsl_table * list mutual_inductive_body)
-                     }.
+
+
+Class Translation :=
+  { tsl_id : ident -> ident ;
+    tsl_tm : tsl_context -> term -> tsl_result term ;
+    tsl_ty : option (tsl_context -> term -> tsl_result term) ;
+
+    (* string = ModPath in which the inductive will be declared *)
+    tsl_ind : tsl_context -> string -> kername -> mutual_inductive_body
+              -> tsl_result (tsl_table * list mutual_inductive_body) }.
 
 
 Definition tsl_ident (id : ident) : ident := (id ++ "ᵗ")%string.
@@ -72,43 +81,65 @@ Definition tsl_name tsl_ident n :=
   end.
 
 
+Definition tmDebug {A} : A -> TemplateMonad unit
+  := tmPrint.
+  (* := fun _ => ret tt. *)
 
-Definition tTranslate {tsl : Translation} (ΣE : tsl_context) (id : ident)
+
+Definition Translate {tsl : Translation} (ΣE : tsl_context) (id : ident)
   : TemplateMonad tsl_context :=
+  tmDebug ("Translate" ++ id);;
   gr <- tmAbout id ;;
-  id' <- tmEval all (tsl_id id) ;;
-  mp <- tmCurrentModPath tt ;;
-  kn' <- tmEval all (mp ++ "." ++ id') ;;
+  tmDebug gr ;;
   match gr with
   | None => fail_nf (id ++ " not found")
   | Some (ConstructRef (mkInd kn n) _)
   | Some (IndRef (mkInd kn n)) =>
-      d <- tmQuoteInductive id ;;
-      d' <- tmEval lazy (tsl_ind ΣE kn kn' d) ;;
-      match d' with
-      | Error e => print_nf e ;; fail_nf ("Translation error during the translation of the inductive " ++ id)
-      | Success (E, decls) =>
-        monad_fold_left (fun _ e => tmMkInductive' e) decls tt ;;
-        print_nf  (id ++ " has been translated as " ++ id') ;;
-        ret (add_global_decl (InductiveDecl kn d) (fst ΣE), E ++ snd ΣE)%list
-      end
-
+    mp <- tmCurrentModPath tt ;;
+    d <- tmQuoteInductive id ;;
+    d' <- tmEval lazy (tsl_ind ΣE mp kn d) ;;
+    match d' with
+    | Error e =>
+      print_nf e ;;
+      fail_nf ("Translation error during the translation of the inductive " ++ id)
+    | Success (E, decls) =>
+      monad_iter tmMkInductive' decls ;;
+      let Σ' := add_global_decl (InductiveDecl kn d) (fst ΣE) in
+      let E' := (E ++ (snd ΣE))%list in
+      Σ' <- tmEval lazy Σ' ;;
+      E' <- tmEval lazy E' ;;
+      print_nf  (kn ++ " has been translated.") ;;
+      ret (Σ', E')
+    end
+    
   | Some (ConstRef kn) =>
     e <- tmQuoteConstant kn true ;;
     match e with
-    | ParameterEntry _ => fail_nf (id ++ "is an axiom, not a definition")
+    | ParameterEntry _ =>
+      fail_nf (id ++ " is an axiom, not a definition. Use Implement Existing.")
     | DefinitionEntry {| definition_entry_type := A;
                          definition_entry_universes := univs;
                          definition_entry_body := t |} =>
+      tmDebug t ;;
       t' <- tmEval lazy (tsl_tm ΣE t) ;;
+      tmDebug t' ;;
       match t' with
-      | Error e => print_nf e ;; fail_nf ("Translation error during the translation of the body of " ++ id)
+      | Error e =>
+        print_nf e ;;
+        fail_nf ("Translation error during the translation of the body of " ++ id)
       | Success t' =>
+        id' <- tmEval all (tsl_id id) ;;
+            tmDebug "here" ;;
+            tmDebug id' ;;
+            tmDebug t' ;;
         tmMkDefinition id' t' ;;
+            tmDebug "doneu" ;;
         let decl := {| cst_universes := univs;
                        cst_type := A; cst_body := Some t |} in
         let Σ' := add_global_decl (ConstantDecl kn decl) (fst ΣE) in
-        let E' := (ConstRef kn, tConst kn' []) :: (snd ΣE) in
+        let E' := (ConstRef kn, tConst id' []) :: (snd ΣE) in
+        Σ' <- tmEval lazy Σ' ;;
+        E' <- tmEval lazy E' ;;
         print_nf  (id ++ " has been translated as " ++ id') ;;
         ret (Σ', E')
       end
@@ -116,58 +147,243 @@ Definition tTranslate {tsl : Translation} (ΣE : tsl_context) (id : ident)
   end.
 
 
-
-Definition tImplement {tsl : Translation} (ΣE : tsl_context)
+Definition Implement {tsl : Translation} (ΣE : tsl_context)
            (id : ident) (A : Type)
   : TemplateMonad (tsl_context) :=
-  tA <- tmQuote A ;;
+  tA  <- tmQuote A ;;
+  match tsl_ty with
+  | None => tmFail "No implementation of tsl_ty provided for this translation."
+  | Some tsl_ty => 
   tA' <- tmEval lazy (tsl_ty ΣE tA) ;;
+  print_nf tA' ;;
   match tA' with
-  | Error e => print_nf e ;; fail_nf ("Translation error during the translation of the type of " ++ id)
+  | Error e =>
+    print_nf e ;;
+    tmFail "Translation error during the translation of the type."
   | Success tA' =>
-    id' <- tmEval all (tsl_id id) ;;
-    let ty := Type in
-    A' <- tmUnquoteTyped ty tA' ;;
-     tmLemma id' (A' : ty) ;;
-     tmAxiom id A ;;
-     gr <- tmAbout id ;;
-     match gr with
-     | Some (ConstRef kn) =>
-       let decl := {| cst_universes := Monomorphic_ctx UContext.empty;
-                      cst_type := tA; cst_body := None |} in
-       let Σ' := add_global_decl (ConstantDecl kn decl) (fst ΣE) in
-       let E' := (ConstRef kn, tConst id' []) :: (snd ΣE) in
-       print_nf (id ++ " has been translated as " ++ id') ;;
-       ret (Σ', E')
-     | _ => fail_nf (id ++ " was not found or is not a constant, this is a bug")
-     end
+      id' <- tmEval all (tsl_id id) ;;
+      tmBind (tmUnquoteTyped Type tA') (fun A' =>
+      tmLemma id' A' ;;
+      tmAxiom id A ;;
+      gr <- tmAbout id ;;
+      match gr with
+      | Some (ConstRef kn) =>
+        let decl := {| cst_universes := Monomorphic_ctx UContext.empty;
+                       cst_type := tA; cst_body := None |} in
+        let Σ' := add_global_decl (ConstantDecl kn decl) (fst ΣE) in
+        let E' := (ConstRef kn, tConst id' []) :: (snd ΣE) in
+        print_nf (id ++ " has been translated as " ++ id') ;;
+        ret (Σ', E')
+      | _ => fail_nf (id ++ " was not found or is not a constant. This is a bug.")
+      end)
+  end
+  end.
+
+Definition body_constant_entry (e : constant_entry) : option term :=
+  match e with
+  | ParameterEntry _ => None
+  | DefinitionEntry {| definition_entry_body := t |} => Some t
   end.
 
 
-(* Definition tImplementExisting (tsl_id : ident -> ident) *)
-(*            (tsl_tm tsl_ty : global_context -> tsl_table -> term *)
-(*                             -> tsl_result term) *)
-(*            (Σ : tsl_context) (id : ident) *)
-(*   : TemplateMonad (option tsl_context) := *)
-(*   e <- tmQuoteConstant id true ;; *)
-(*   match e with *)
-(*   | ParameterEntry _ => tmPrint "Not a definition" ;; *)
-(*                        tmReturn None *)
-(*   | DefinitionEntry {| definition_entry_type := A; *)
-(*                        definition_entry_body := t |} => *)
-(*     match tsl_ty (fst Σ) (snd Σ) A with *)
-(*     | Error _ => tmPrint "tsl error in type" ;; *)
-(*                   tmReturn None *)
-(*     | Success tA' => *)
-(*       id' <- tmEval all (tsl_id id) ;; *)
-(*       A' <- tmUnquoteTyped Type tA' ;; *)
-(*       tmLemma id' A' ;; *)
-(*       let decl := {| cst_universes := []; *)
-(*                      cst_type := A; cst_body := Some t |} in *)
-(*       let Σ' := ConstantDecl id decl :: (fst Σ) in *)
-(*       let E' := (ConstRef id, tConst id' []) :: (snd Σ) in *)
-(*       msg <- tmEval all (id ++ " has been translated as " ++ id') ;; *)
-(*       tmPrint msg ;; *)
-(*       tmReturn (Some (Σ', E')) *)
-(*     end *)
-(*   end. *)
+Definition ImplementExisting {tsl : Translation} (ΣE : tsl_context) (id : ident)
+  : TemplateMonad tsl_context :=
+  gr <- tmAbout id ;;
+  id' <- tmEval all (tsl_id id) ;;
+  mp <- tmCurrentModPath tt ;;
+  match tsl_ty with
+  | None => tmFail "No implementation of tsl_ty provided for this translation."
+  | Some tsl_ty => 
+  match gr with
+  | None => fail_nf (id ++ " not found")
+  | Some (ConstRef kn) =>
+    e <- tmQuoteConstant kn true ;;
+    match e with
+    | ParameterEntry  {| parameter_entry_type := A  |}
+    | DefinitionEntry {| definition_entry_type := A |} =>
+      tmDebug "plop1" ;;
+      ΣE <- tmEval lazy ΣE ;;
+      tmDebug ΣE ;;
+      tA' <- tmEval lazy (tsl_ty ΣE A) ;;  (* long *)
+      tmDebug "plop" ;;
+      match tA' with
+      | Error e =>
+        print_nf e ;;
+        fail_nf ("Translation error during the translation of the type of " ++ id)
+      | Success tA' =>
+        tmDebug "plop2" ;;
+        tmBind (tmUnquoteTyped Type tA') (fun A' =>
+        tmDebug "plop3" ;;
+        tmLemma id' A' ;;
+        let decl := {| cst_universes := Monomorphic_ctx UContext.empty;
+                       cst_type := A; cst_body := body_constant_entry e |} in
+        let Σ' := add_global_decl (ConstantDecl kn decl) (fst ΣE) in
+        let E' := (ConstRef kn, tConst id' []) :: (snd ΣE) in
+        print_nf (id ++ " has been translated as " ++ id') ;;
+        ret (Σ', E'))
+      end
+    end
+  | Some (IndRef (mkInd kn n)) =>
+    d <- tmQuoteInductive kn ;;
+    match List.nth_error (ind_bodies d) n with
+      | None => fail_nf ("The declaration of "
+                          ++ id ++ " has not enough bodies. This is a bug.")
+      | Some {| ind_type := A |} => 
+      tA' <- tmEval lazy (tsl_ty ΣE A) ;;
+      match tA' with
+      | Error e =>
+        print_nf e ;;
+        fail_nf ("Translation error during the translation of the type of " ++ id)
+      | Success tA' =>
+        id' <- tmEval all (tsl_id id) ;;
+        tmBind (tmUnquoteTyped Type tA') (fun A' =>
+        tmLemma id' A' ;;
+        let Σ' := add_global_decl (InductiveDecl kn d) (fst ΣE) in
+        let E' := (IndRef (mkInd kn n), tConst id' []) :: (snd ΣE) in
+        print_nf (id ++ " has been translated as " ++ id') ;;
+        ret (Σ', E'))
+      end
+    end
+
+  | Some (ConstructRef (mkInd kn n) k) =>
+    d <- tmQuoteInductive kn ;;
+    tmDebug "plop1" ;;
+    match List.nth_error (ind_bodies d) n with
+    | None => fail_nf ("The declaration of "
+                        ++ id ++ " has not enough bodies. This is a bug.")
+    | Some {| ind_ctors := ctors |} => 
+      tmDebug "plop2" ;;
+      match List.nth_error ctors k with
+      | None => fail_nf ("The body of "
+                          ++ id ++ " has not enough constructors. This is a bug.")
+      | Some (_, ty, _) =>  (* keep id? *)
+        tmDebug "plop3" ;;
+        let A := substl (inds kn [] (* FIXME uctx *) (ind_bodies d)) ty in
+        tmDebug "plop4" ;;
+        tA' <- tmEval lazy (tsl_ty ΣE A) ;;
+        tmDebug "plop5" ;;
+        match tA' with
+        | Error e =>
+          print_nf e ;;
+          fail_nf ("Translation error during the translation of the type of " ++ id)
+        | Success tA' =>
+          tmDebug "plop6" ;;
+          id' <- tmEval all (tsl_id id) ;;
+          tmBind (tmUnquoteTyped Type tA') (fun A' =>
+          tmDebug "plop7" ;;
+          tmLemma id' A' ;;
+          let E' := (ConstructRef (mkInd kn n) k, tConst id' []) :: (snd ΣE) in
+          print_nf (id ++ " has been translated as " ++ id') ;;
+          ret (fst ΣE, E'))
+        end
+      end
+    end
+  end
+  end.
+
+
+
+Require Import Ascii.
+
+Fixpoint string_of_ascii_list l :=
+  match l with
+  | nil => EmptyString
+  | a :: s => String a (string_of_ascii_list s)
+  end.
+
+Definition string_of_ascii_list_rev l := string_of_ascii_list (rev l).
+
+(* Compute (string_of_ascii_list_rev ["."; "g"; "h"]%char). *)
+
+
+(* empty list on empty string ?? *)
+(* acc is in reverse order *)
+Fixpoint split_string_aux (sep : ascii) (s : string) (acc : list ascii)
+  : list string :=
+  match s with
+  | EmptyString => [string_of_ascii_list_rev acc]
+  | String a s => if Ascii.ascii_dec a sep then (string_of_ascii_list_rev acc)
+                                                 :: (split_string_aux sep s [])
+                 else split_string_aux sep s (a :: acc)
+  end.
+
+Definition split_string (sep : Ascii.ascii) (s : string) : list string :=
+  split_string_aux sep s [].
+
+(* Compute (split_string "."%char "eopjqd.qS.E"). *)
+(* Compute (split_string "."%char ""). *)
+
+Definition ident_of_kn (kn : kername) : ident
+  := last (split_string "."%char kn) kn.
+
+Definition tsl_kn (tsl_ident : ident -> ident) (kn : kername) mp
+  := mp ++ "." ++ (tsl_ident (ident_of_kn kn)).
+
+
+
+Definition TranslateRec {tsl : Translation} (ΣE : tsl_context) {A} (t : A) := 
+  p <- tmQuoteRec t ;;
+  tmPrint "~~~~~~~~~~~~~~~~~~" ;;
+  monad_fold_left (fun ΣE decl =>
+    print_nf ("Translating " ++ global_decl_ident decl) ;;
+    match decl with
+    | ConstantDecl kn decl =>
+      match lookup_tsl_table (snd ΣE) (ConstRef kn) with
+      | Some _ => print_nf (kn ++ " was already translated") ;; ret ΣE
+      | None => 
+        match decl with
+        | {| cst_body := None |} =>
+          fail_nf (kn ++ " is an axiom. Use Implement Existing.")
+                    
+        | {| cst_type := A; cst_body := Some t; cst_universes := univs |} =>
+          tmDebug "go";;
+          t' <- tmEval lazy (tsl_tm ΣE t) ;;
+          tmDebug "done";;
+          match t' with
+          | Error e =>
+            print_nf e ;;
+            fail_nf ("Translation error during the translation of the body of "
+                       ++ kn)
+          | Success t' =>
+            let id := ident_of_kn kn in
+            let id' := tsl_ident id in
+            tmDebug "here";;
+            tmDebug id' ;;
+            tmDebug t' ;;
+            tmMkDefinition id' t' ;;
+            tmDebug "there";;
+            let Σ' := add_global_decl (ConstantDecl kn decl) (fst ΣE) in
+            let E' := (ConstRef kn, tConst id' []) :: (snd ΣE) in
+            Σ' <- tmEval lazy Σ' ;;
+            E' <- tmEval lazy E' ;;
+            print_nf  (id ++ " has been translated as " ++ id') ;;
+            ret (Σ', E')
+          end
+        end
+      end
+
+    | InductiveDecl kn d => 
+      match lookup_tsl_table (snd ΣE) (IndRef (mkInd kn 0)) with
+      | Some _ => print_nf (kn ++ " was already translated") ;; ret ΣE
+      | None => 
+        tmDebug "go'";;
+        mp <- tmCurrentModPath tt ;;
+        d' <- tmEval lazy (tsl_ind ΣE mp kn d) ;;
+        tmDebug "done'";;
+         match d' with
+         | Error e => 
+           print_nf e ;;
+           fail_nf ("Translation error during the translation of the inductive "
+                      ++ kn)
+         | Success (E, decls) =>
+           monad_iter tmMkInductive' decls ;;
+           let Σ' := add_global_decl (InductiveDecl kn d) (fst ΣE) in
+           let E' := (E ++ (snd ΣE))%list in
+           Σ' <- tmEval lazy Σ' ;;
+           E' <- tmEval lazy E' ;;
+           print_nf  (kn ++ " has been translated.") ;;
+           ret (Σ', E')
+         end
+      end
+    end)
+  (fst p) ΣE.
