translations/sigma.v
@@ -10,13 +10,14 @@ Arguments π1 {A B} _.
 Arguments π2 {A B} _.
 Arguments mk_sig {A B} _ _.
 
-Notation "{ t : A & P }" := (sigma A (fun t => P)) : type_scope.
+Notation "{ x  &&  P }" := (sigma (fun x => P)) : type_scope.
+Notation "{ t : A && P }" := (sigma A (fun t => P)) : type_scope.
 Notation "( x ; y )" := (mk_sig x y) : sigma_scope.
-Notation "x .1" := (π1 x) (at level 2, left associativity, format "x '.1'") : sigma_scope.
-Notation "x .2" := (π2 x) (at level 2, left associativity, format "x '.2'") : sigma_scope.
-Notation "'exists' x .. y , p" := (sigma _ (fun x => .. (sigma _ (fun y => p)) ..))
+Notation "x .1" := (π1 x) (at level 3, format "x '.1'") : sigma_scope.
+Notation "x .2" := (π2 x) (at level 3, format "x '.2'") : sigma_scope.
+Notation "'∃' x .. y , p" := (sigma _ (fun x => .. (sigma _ (fun y => p)) ..))
   (at level 200, x binder, right associativity,
-   format "'[' 'exists'  '/  ' x  ..  y ,  '/  ' p ']'")
+   format "'[' '∃'  '/  ' x  ..  y ,  '/  ' p ']'")
                                   : type_scope.
 
 Notation " A × B " := (sigma A (fun _ => B)) (at level 30) : type_scope.
