translations/times_bool2.v
@@ -1,0 +1,195 @@
+Require Import Template.All.
+Import String Lists.List.ListNotations MonadNotation.
+Open Scope list_scope. Open Scope string_scope.
+Require Import translation_utils times_bool_fun MiniHoTT.
+Require Import TypingFlags.Loader.
+Print Typing Flags.
+
+Run TemplateProgram (TC <- ImplementExisting emptyTC "paths" ;;
+                     TC <- ImplementExisting TC "idpath" ;;
+                     TC <- ImplementExisting TC "paths_ind" ;;
+                     TC <- ImplementExisting TC "transport" ;;
+                     TC <- ImplementExisting TC "sigT" ;;
+                     TC <- ImplementExisting TC "projT1" ;;
+                     TC <- ImplementExisting TC "projT2" ;;
+                     TC <- ImplementExisting TC "existT" ;;
+                     tmDefinition "eqTC" TC).
+Next Obligation.
+  tIntro A. tIntro x. tIntro y. exact (x = y).
+Defined.
+Next Obligation.
+  tIntro A. tIntro x. exact 1.
+Defined.
+Next Obligation.
+  tIntro A. tIntro a. tIntro P. tIntro t. tIntro y. tIntro p.
+  exact (paths_ind a (fun y p => π1 (π1 P y) p) t y p).
+Defined.
+Next Obligation.
+  tIntro A. tIntro P. tIntro x. tIntro y. tIntro p. tIntro t.
+  exact (transport (π1 P) p t).
+Defined.
+Next Obligation.
+  tIntro A. tIntro B. exact (sigT (π1 B)).
+Defined.
+Next Obligation.
+  tIntro A. tIntro B. tIntro u. exact u.1.
+Defined.
+Next Obligation.
+  tIntro A. tIntro B. tIntro u. exact u.2.
+Defined.
+Next Obligation.
+  tIntro A. tIntro B. tIntro x. tIntro y. exact (x; y).
+Defined.
+
+Definition isequiv {A B} (f : A -> B) :=
+  exists (g : B -> A) (H1 : forall x, paths (g (f x)) x), (forall y, paths (f (g y)) y).
+
+Definition idequiv A : @isequiv A A (fun x => x).
+  unshelve econstructor. exact (fun y => y).
+  split; intro; exact 1.
+Defined.
+
+Definition equiv A B := exists f, @isequiv A B f.
+
+Definition coe {A B} (p : A = B) : A -> B
+  := transport idmap p.
+
+Definition transport_pV {A : Type} (P : A -> Type) {x y : A} (p : x = y)
+  : forall z : P y, p # p^ # z = z
+  := paths_ind x (fun y p => forall z : P y, p # p^ # z = z) (fun z => 1) y p.
+
+Definition transport_Vp {A : Type} (P : A -> Type) {x y : A} (p : x = y)
+  : forall z : P x, p^ # p # z = z
+  := paths_ind x (fun y p => forall z : P x, p^ # p # z = z) (fun z => 1) y p.
+
+Definition id2equiv A B (p : A = B) : equiv A B.
+  repeat unshelve econstructor.
+  exact (transport idmap p).
+  exact (transport idmap p^).
+  all: unfold coe; intro.
+  (* refine (paths_ind A (fun y p => forall z : A, p^ # p # z = z) (fun z => 1) B p _). *)
+  (* refine (paths_ind A (fun y p => forall z : y, p # p^ # z = z) (fun z => 1) B p _). *)
+  exact (transport_Vp idmap _ _).
+  exact (transport_pV idmap _ _).
+Defined.
+
+Definition UA := forall A B, isequiv (id2equiv A B).
+
+Run TemplateProgram (TC <- Translate eqTC "isequiv" ;;
+                     TC <- Translate TC "equiv" ;;
+                     TC <- ImplementExisting TC "eq" ;;
+                     TC <- Translate TC "inverse" ;;
+                     tmDefinition "eqTC2" TC).
+Next Obligation.
+  tIntro A. tIntro x. tIntro y. exact (@eq A x y).
+Defined.
+
+
+Fail Run TemplateProgram (TC <- TranslateRec eqTC2 (UA -> False) ;;
+                     tmDefinition "eqTC'" TC ;;
+                     Implement TC "notUA" (UA -> False)).
+
+
+Run TemplateProgram (TC <- Translate eqTC "isequiv" ;;
+                     tmDefinition "eqTC2" TC).
+
+Run TemplateProgram (TC <- Translate eqTC2 "equiv" ;;
+                     tmDefinition "eqTC2'" TC).
+
+
+Definition contr A := exists x : A, forall y, x = y.
+Definition weakFunext
+  := forall (A : Type) (P : A -> Type), (forall x, contr (P x)) -> contr (forall x, P x).
+
+Run TemplateProgram (TC <- Translate eqTC2 "contr" ;;
+                     TC <- Translate TC "weakFunext" ;;
+                     tmDefinition "eqTC3" TC).
+
+Goal weakFunextᵗ -> False.
+  intro H. tSpecialize H unit. tSpecialize H (pair (fun _ => unit) true).
+  simple refine (let H' := π1 H _ in _).
+  - tIntro x. lazy. exists tt. tIntro y; now destruct y.
+  - lazy in H'. destruct H' as [H1 H2]; clear H.
+    tSpecialize H2 (pair (π1 H1) (negb (π2 H1))).
+    apply (f_equal π2) in H2. lazy in H2.
+    set (π2 H1) in H2. change (b = negb b) in H2.
+    destruct b; inversion H2.
+Defined.
+
+Definition retract A B := exists (f : A -> B) (g : B -> A), g o f == idmap.
+
+Definition contr_retract {A B} (R : retract A B) (C : contr B) : contr A.
+  destruct R as [f [g e]].
+  exists (g C.1). intro y.
+  refine (ap g _ @ e y).
+  exact (C.2 (f y)).
+Defined.
+
+Definition postcompose_equiv
+  := forall A B (e : equiv A B) A', isequiv (fun (g : A' -> A) => e.1 o g).
+
+Definition UA_postcomposeequiv : UA -> postcompose_equiv.
+  (* uses eta *)
+Admitted.
+
+Definition α {A} (P : A -> Type) := fun (g : A -> sigT P) => pr1 o g.
+
+Definition contr_isequivα := forall A P, (forall x, contr (P x)) -> isequiv (@α A P).
+
+Definition postcomposeequiv_αequiv
+  : postcompose_equiv -> contr_isequivα.
+  (* no eta ? *)
+  intros H A P C.
+  refine (H (sigT P) A (_; _) _).
+  unshelve econstructor.
+  exact (fun x => (x; (C x).1)).
+  lazy. econstructor.
+  intros [x y]. refine (path_sigma' P 1 _). exact ((C x).2 y).
+  intro; exact 1.
+Defined.
+
+Definition fib {A B} (f : A -> B) y := exists x, f x = y.
+
+Definition equiv_contrfib {A B} (f : A -> B) (Hf : isequiv f) y : contr (fib f y).
+Admitted.
+
+Definition contr_retractα
+  := forall A P, (forall x, contr (P x)) -> retract (forall x : A, P x) (fib (α P) idmap).
+
+Definition contr_retract_α : contr_retractα.
+  intros A P H.
+  simple refine (_; (_; _)).
+  - intro f. exists (fun x => (x; f x)). exact 1.
+  - intros [g p] x. refine (_ # (g x).2).
+    exact (ap10 p x).
+  - intro f; lazy. exact 1. (* uses eta! *)
+Defined. 
+
+(* Run TemplateProgram (TC <- TranslateRec eqTC3 contr_retractα ;; *)
+(*                      TC <- ImplementExisting TC "contr_retract_α" ;; *)
+(*                      tmDefinition "eqTC4" TC). *)
+(* Next Obligation. *)
+(*   tIntro A. tIntro P. tIntro H. *)
+(*   simple refine (_; (_; _)). *)
+(*   - tIntro f. exists (pair (fun x => (x; π1 f x)) (π2 f)). exact 1. *)
+(*   - tIntro gp. refine (pair (fun x => _) (π2 gp.1)). *)
+(*     refine (_ # ((π1 gp.1) x).2). all: lazy. *)
+(*     exact (ap10 (ap π1 gp.2) x). *)
+(*   - tIntro f; lazy. exact 1. *)
+(* Defined. *)
+
+Definition UA_postcomposeequiv' : UA -> postcompose_equiv.
+  intros ua A B e X. repeat unshelve econstructor.
+  - intros f x. exact (e.2.1 (f x)).
+  - intro f.
+
+  (* uses eta *)
+Admitted.
+
+
+Definition αequiv_weakfunext : contr_isequivα -> weakFunext.
+  intros Hα A P H.
+  refine (contr_retract _ _).
+  2: exact (equiv_contrfib _ (Hα A P H) idmap).
+  exact (contr_retract_α A P H).
+Defined.
