translations/times_bool_fun.v
@@ -1,0 +1,380 @@
+Require Import Template.All.
+From Translations Require Import translation_utils MiniHoTT.
+Import String Lists.List.ListNotations MonadNotation.
+Open Scope list_scope. Open Scope string_scope.
+
+Unset Strict Unquote Universe Mode.
+
+Set Primitive Projections.
+Record prod A B := pair { π1 : A ; π2 : B }.
+
+Arguments π1 {_ _} _.
+Arguments π2 {_ _} _.
+Arguments pair {_ _} _ _.
+
+Notation "( x ; y )" := (pair x y) : prod_scope.
+Notation " A × B " := (prod A B) (at level 30) : type_scope.
+Open Scope prod_scope.
+
+Quote Definition tprod := prod.
+Quote Definition tpair := @pair.
+Definition prod_ind := Eval compute in
+  match tprod with tInd i _ => i | _ => mkInd "bug: prod not an inductive" 0 end.
+Definition proj1 (t : term) : term
+  := tProj (prod_ind, 2, 0) t.
+Definition proj2 (t : term) : term
+  := tProj (prod_ind, 2, S 0) t.
+
+Quote Definition tbool := bool.
+Quote Definition ttrue := true.
+Definition timesBool (A : term) := tApp tprod [A; tbool].
+Definition pairTrue typ tm := tApp tpair [typ; tbool; tm; ttrue].
+
+
+
+
+Local Instance tit : config.checker_flags := {| config.check_univs := false |}.
+
+Fixpoint tsl_rec (fuel : nat) (Σ : global_context) (E : tsl_table) (Γ : context) (t : term) {struct fuel}
+  : tsl_result term :=
+  match fuel with
+  | O => raise NotEnoughFuel
+  | S fuel =>
+  match t with
+  | tRel  n => ret (tRel n)
+  | tSort s => ret (tSort s)
+
+  | tCast t c A => t' <- tsl_rec fuel Σ E Γ t ;;
+                  A' <- tsl_rec fuel Σ E Γ A ;;
+                  ret (tCast t' c A')
+
+  | tProd n A B => A' <- tsl_rec fuel Σ E Γ A ;;
+                  B' <- tsl_rec fuel Σ E (Γ ,, vass n A) B ;;
+                  ret (timesBool (tProd n A' B'))
+
+  | tLambda n A t => A' <- tsl_rec fuel Σ E Γ A ;;
+                    t' <- tsl_rec fuel Σ E (Γ ,, vass n A) t ;;
+                    match infer Σ (Γ ,, vass n A) t with
+                    | Checked B =>
+                      B' <- tsl_rec fuel Σ E (Γ ,, vass n A) B ;;
+                      ret (pairTrue (tProd n A' B') (tLambda n A' t'))
+                    | TypeError t => raise (TypingError t)
+                    end
+
+  | tLetIn n t A u => t' <- tsl_rec fuel Σ E Γ t ;;
+                     A' <- tsl_rec fuel Σ E Γ A ;;
+                     u' <- tsl_rec fuel Σ E (Γ ,, vdef n t A) u ;;
+                     ret (tLetIn n t' A' u')
+
+  | tApp t us => t' <- tsl_rec fuel Σ E Γ t ;;
+                monad_fold_left (fun t u => u' <- tsl_rec fuel Σ E Γ u ;;
+                                         ret (tApp (proj1 t) [u'])) us t'
+
+  | tConst s univs => lookup_tsl_table' E (ConstRef s)
+  | tInd i univs => lookup_tsl_table' E (IndRef i)
+  | tConstruct i n univs => lookup_tsl_table' E (ConstructRef i n)
+  | tProj p t => t' <- tsl_rec fuel Σ E Γ t ;;
+                ret (tProj p t')
+
+  | tFix bodies n =>
+    Γ' <- monad_map (fun '{| dname := na; dtype := ty; dbody := b; rarg := r |} =>
+                      ty' <- tsl_rec fuel Σ E Γ ty ;;
+                      ret {| decl_name := na; decl_body := None; decl_type := ty'|})
+                   bodies;;
+    bodies' <- monad_map (fun '{| dname := na; dtype := ty; dbody := b; rarg := r |} =>
+                           ty' <- tsl_rec fuel Σ E Γ ty ;;
+                           b'  <- tsl_rec fuel Σ E (Γ ++ Γ')%list b ;;
+                           ret {| dname := na; dtype := ty';
+                                  dbody := b'; rarg := r |})
+                        bodies ;;
+    ret (tFix bodies' n)
+  | _ => raise TranslationNotHandeled (* var evar meta case cofix *)
+  end
+  end.
+
+
+(* Definition recompose_prod (nas : list name) (ts : list term) (u : term) *)
+(*   : term *)
+(*   := let nats := List.combine nas ts in *)
+(*      List.fold_right (fun t u => tProd (fst t) (snd t) u) u nats. *)
+
+Definition combine' {A B} (p : list A * list B) : list (A * B)
+  := List.combine  (fst p) (snd p).
+
+
+Fixpoint replace pat u t {struct t} :=
+  if eq_term uGraph.init_graph t pat then u else
+    match t with
+    | tCast t c A => tCast (replace pat u t) c (replace pat u A)
+    | tProd n A B => tProd n (replace pat u A) (replace (up pat) (up u) B)
+    | tLambda n A t => tLambda n (replace pat u A) (replace (up pat) (up u) t)
+    | tLetIn n t A B => tLetIn n (replace pat u t) (replace pat u A)
+                              (replace (up pat) (up u) B)
+    | tApp t us => tApp (replace pat u t) (List.map (replace pat u) us)
+    | tProj p t => tProj p (replace pat u t)
+    | _ => t (* todo *)
+    end.
+
+
+(* If tm of type typ = Π [A0] [A1] ... . [B], returns *)
+(* a term of type [Π A0 A1 ... . B] *)
+Definition pouet (tm typ : term) : term.
+  simple refine (let '((names, types), last) := decompose_prod typ in
+                 let L' := List.fold_left _ (List.combine names types) [] in _).
+  exact (fun Γ' A => Γ' ,, vass (fst A) (snd A)).
+  refine (let args := fold_left_i (fun l i _ => tRel i :: l) L' [] in _).
+  refine (fst (List.fold_left _ L' (subst_app tm args, last))).
+  refine (fun '(tm, typ) decl =>
+            let A := tProd decl.(decl_name) decl.(decl_type) typ in
+            (pairTrue A (tLambda decl.(decl_name) decl.(decl_type) tm),
+             timesBool A)).
+Defined.
+
+
+
+Definition tsl_mind_body (ΣE : tsl_context) (mp : string) (kn : kername)
+           (mind : mutual_inductive_body)
+  : tsl_result (tsl_table * list mutual_inductive_body).
+  refine (let tsl := fun Γ t => match tsl_rec fuel (fst ΣE) (snd ΣE) Γ t with
+                             | Success x => x
+                             | Error _ => todo
+                             end in
+          let kn' := tsl_kn tsl_ident kn mp in _).
+  refine (let LI := List.split (map_i _ mind.(ind_bodies)) in
+          ret (List.concat (fst LI),
+               [{| ind_npars := mind.(ind_npars);
+                   ind_bodies := snd LI;
+                   ind_universes := mind.(ind_universes)|}])). (* FIXME always ok? *)
+  intros i ind.
+  simple refine (let ind_type' := _ in
+                 let ctors' := List.split (map_i _ ind.(ind_ctors)) in
+                 (_ :: fst ctors',
+                  {| ind_name := tsl_ident ind.(ind_name);
+                     ind_type := ind_type';
+                     ind_kelim := ind.(ind_kelim);
+                     ind_ctors := snd ctors';
+                     ind_projs := [] |})).
+  + (* arity *)
+    refine (let L := decompose_prod ind.(ind_type) in _).
+    simple refine (let L' := List.fold_left _ (combine' (fst L)) [] in _).
+    exact (fun Γ' A => Γ' ,, vass (fst A) (tsl Γ' (snd A))).
+    refine (List.fold_left _ L' (snd L)).
+    exact (fun t decl => tProd decl.(decl_name) decl.(decl_type) t).
+  + (* constructors *)
+    intros k ((name, typ), nargs).
+    simple refine (let ctor_type' := _ in
+                   ((ConstructRef (mkInd kn i) k,
+                     pouet (tConstruct (mkInd kn' i) k []) _),
+                    (tsl_ident name, ctor_type', nargs))).
+    * refine (fold_left_i (fun t i _ => replace (proj1 (tRel i)) (tRel i) t)
+                          mind.(ind_bodies) _).
+      refine (let L := decompose_prod typ in _).
+      simple refine (let L' := List.fold_left _ (combine' (fst L))
+                                              [] in _).
+      exact (fun Γ' A => Γ' ,, vass (fst A) (tsl Γ' (snd A))).
+      refine (List.fold_left _ L' _).
+      exact (fun t decl => tProd decl.(decl_name) decl.(decl_type) t).
+      exact (match snd L with
+             | tApp t us => tApp t (List.map (tsl L') us)
+             | _ as t => t
+             end).
+    * refine (fold_left_i (fun t l _ => replace (tRel l) (tInd (mkInd kn' i) []) t)
+                          mind.(ind_bodies) ctor_type').
+  + (* table *)
+    refine (IndRef (mkInd kn i), pouet (tInd (mkInd kn' i) []) ind_type').
+Defined.
+
+
+Fixpoint refresh_universes (t : term) {struct t} :=
+  match t with
+  | tSort s => tSort (if Universe.is_level s then s else [])
+  | tProd na b t => tProd na b (refresh_universes t)
+  | tLetIn na b t' t => tLetIn na b t' (refresh_universes t)
+  | tCast x x0 x1 => tCast (refresh_universes x) x0 (refresh_universes x1)
+  | tLambda x x0 x1 => tLambda x (refresh_universes x0) (refresh_universes x1)
+  | tApp x x0 => tApp (refresh_universes x) (List.map refresh_universes x0)
+  | tProj x x0 => tProj x (refresh_universes x0)
+  | _ => t
+  end.
+
+Instance tsl_fun : Translation
+  := {| tsl_id := tsl_ident ;
+        tsl_tm := fun ΣE t => t' <- tsl_rec fuel (fst ΣE) (snd ΣE) [] t ;;
+                           ret (refresh_universes t');
+        tsl_ty := Some (fun ΣE t => t' <- tsl_rec fuel (fst ΣE) (snd ΣE) [] t ;;
+                                 ret (refresh_universes t')) ;
+        tsl_ind := tsl_mind_body |}.
+
+
+Tactic Notation "tSpecialize" ident(H) uconstr(t)
+  := apply π1 in H; specialize (H t).
+Tactic Notation "tIntro" ident(H)
+  := refine (fun H => _; true).
+
+Definition NotFunext :=
+  ((forall (A B : Set) (f g : A -> B), (forall x:A, f x = g x) -> f = g) -> False).
+
+Run TemplateProgram (TC <- TranslateRec emptyTC NotFunext ;;
+                     tmDefinition "TC" TC ;;
+                     Implement TC "notFunext" NotFunext).
+Next Obligation. 
+  unfold NotFunextᵗ; cbn in *.
+  tIntro H. 
+  tSpecialize H unit. tSpecialize H unit. 
+  tSpecialize H (fun x => x; true). tSpecialize H (fun x => x; false). 
+  tSpecialize H (fun x => eq_reflᵗ _ _; true).
+  inversion H. 
+Defined.
+
+Run TemplateProgram (Implement TC "notη" ((forall (A B : Set) (f : A -> B), f = fun x => f x) -> False)).
+
+Next Obligation.
+  tIntro H. 
+  tSpecialize H unit. tSpecialize H unit. 
+  tSpecialize H (fun x => x; false). cbn in H.
+  inversion H. 
+Defined.
+
+(* Require Import Vector Even. *)
+(* Definition SS := S. *)
+(* Run TemplateProgram (TC <- Translate emptyTC "nat" ;; *)
+(*                      TC <- Translate TC "even" ;; *)
+(*                      tmDefinition "TC2" TC). *)
+
+(* Inductive foo := *)
+(* | bar : (nat -> foo) -> foo. *)
+(* Definition bar' := bar. *)
+(* Run TemplateProgram (TranslateRec TC2 bar'). *)
+
+
+Definition UIP := forall A (x y : A) (p q : x = y), p = q.
+
+
+Run TemplateProgram (tmQuoteRec UIP >>= tmPrint).
+
+Run TemplateProgram (TC <- TranslateRec TC UIP ;;
+                     tmDefinition "eqTC" TC).
+
+Definition eqᵗ_eq {A} x y
+  : eqᵗ A x y -> x = y.
+Proof.
+  destruct 1; reflexivity.
+Defined.
+
+Definition eq_eqᵗ {A} x y
+  : x = y -> eqᵗ A x y.
+Proof.
+  destruct 1; reflexivity.
+Defined.
+
+Definition isequiv_eqᵗ_eq {A} x y
+  : IsEquiv (@eqᵗ_eq A x y).
+Proof.
+  unshelve eapply isequiv_adjointify.
+  apply eq_eqᵗ.
+  all: intros []; reflexivity.
+Defined.
+
+Theorem preserves_UIP : UIP -> UIPᵗ.
+Proof.
+  unfold UIP, UIPᵗ.
+  intros H.
+  tIntro A. tIntro x. tIntro y. tIntro p. tIntro q.
+  cbn in *.
+  apply eq_eqᵗ. refine (equiv_inj _ (H := isequiv_eqᵗ_eq _ _) _).
+  apply H.
+Defined.
+
+
+Definition wFunext
+  := forall A (B : A -> Type) (f g : forall x, B x), (forall x, f x = g x) -> f = g.
+
+
+Run TemplateProgram (TC <- TranslateRec eqTC (wFunext -> False) ;;
+                     tmDefinition "eqTC'" TC ;;
+                     Implement TC "notwFunext" (wFunext -> False)).
+Next Obligation.
+  tIntro H.
+  tSpecialize H unit. tSpecialize H (fun _ => unit; true).
+  tSpecialize H (fun x => x; true). tSpecialize H (fun x => x; false).
+  tSpecialize H (fun x => eq_reflᵗ _ _; true).
+  inversion H.
+Defined.
+
+Definition wUnivalence
+  := forall A B, Equiv A B -> A = B.
+
+Run TemplateProgram (TC <- Translate eqTC' "idpath" ;;
+                     TC <- ImplementExisting TC "paths_ind" ;;
+                     tmDefinition "eqTC''" TC).
+Next Obligation.
+  tIntro A. tIntro a. tIntro P. tIntro t.
+  tIntro y. tIntro p. destruct p. exact t.
+Defined.
+
+Run TemplateProgram (TC <- TranslateRec eqTC'' wUnivalence ;;
+                     tmDefinition "eqTC3" TC).
+
+Theorem preserves_wUnivalence : wUnivalence -> wUnivalenceᵗ.
+Proof.
+  unfold wUnivalence, wUnivalenceᵗ.
+  intros H.
+  tIntro A. tIntro B. tIntro H.
+  cbn in *.
+  apply eq_eqᵗ. apply H0. destruct H as [[f bf] Hf]; cbn in *.
+  exists f. destruct Hf as [[g bg] [s _] [r _] _]; cbn in *.
+  unshelve eapply isequiv_adjointify. assumption.
+  all: intro; apply eqᵗ_eq; auto.
+Defined.
+
+
+
+
+
+
+Definition bool_of_Equivᵗ {A B} (e : Equivᵗ A B) : bool.
+  now destruct e as [[_ b] _].
+Defined.
+
+Definition UA := forall A B, IsEquiv (paths_ind A (fun B _ => Equiv A B) (equiv_idmap A) B).
+
+Run TemplateProgram (TC <- Translate eqTC3 "isequiv_idmap" ;;
+                     TC <- Translate TC "equiv_idmap" ;;
+                     TC <- Translate TC "UA" ;;
+                     tmDefinition "eqTC4" TC).
+
+Axiom fx : Funext.
+Axiom ua : UA.
+
+
+Lemma eqᵗ_unit_unit (e e' : eqᵗ Type unit unit) : e = e'.
+  refine (equiv_inj (eqᵗ_eq _ _) _).
+  - apply isequiv_eqᵗ_eq.
+  - refine (equiv_inj _ (H:=ua _ _) _).
+    apply path_equiv; cbn. apply fx.
+    apply fx. intro; apply path_unit.
+Defined.
+
+
+Run TemplateProgram (Implement eqTC4 "notUA" (UA -> False)).
+Next Obligation.
+  unfold UAᵗ; tIntro ua.
+  tSpecialize ua unit.
+  tSpecialize ua unit.
+  destruct ua as [[g bg] H1 H2 _]; cbn -[paths_indᵗ] in *.
+  simple refine (let e1 := BuildEquivᵗ unit unit (idmap; true) _ in _); cbn. {
+    unshelve econstructor; cbn. exact (idmap; true).
+    all: tIntro x; reflexivity. }
+  simple refine (let e2 := BuildEquivᵗ unit unit (idmap; false) _ in _); cbn. {
+    unshelve econstructor; cbn. exact (idmap; true).
+    all: tIntro x; reflexivity. }
+  assert (e1 = e2). {
+    etransitivity. symmetry. eapply eqᵗ_eq.
+    exact (π1 H1 e1).
+    etransitivity. 2: eapply eqᵗ_eq; exact (π1 H1 e2).
+    clearbody e1 e2; clear.
+    assert (g e1 = g e2). apply eqᵗ_unit_unit.
+    now rewrite X. }
+  apply (f_equal bool_of_Equivᵗ) in X. cbn in X.
+  inversion X.
+Defined.
